%% LyX 2.1.2 created this file.  For more info, see http://www.lyx.org/.
%% Do not edit unless you really know what you are doing.
\documentclass[english]{article}
\usepackage[T1]{fontenc}
\usepackage[latin9]{inputenc}
\usepackage[letterpaper]{geometry}
\geometry{verbose,tmargin=2cm,bmargin=2cm,lmargin=2cm,rmargin=2cm,headheight=1cm,headsep=1cm,footskip=1cm}
\usepackage{fancyhdr}
\pagestyle{fancy}
\setcounter{secnumdepth}{-1}
\usepackage{amsmath}
\usepackage{amssymb}
\usepackage{cancel}
\usepackage{esint}

\makeatletter
%%%%%%%%%%%%%%%%%%%%%%%%%%%%%% User specified LaTeX commands.
\usepackage{pgf}
\usepackage{tikz}
\usepackage{pstricks}
\usepackage{lastpage}

\let\oldmaketitle\maketitle

\renewcommand{\maketitle}{\oldmaketitle \thispagestyle{fancy}}

\makeatother

\usepackage{babel}
\begin{document}

\lhead{Alex Hagen}


\chead{QE Studying: Thermal Hydraulics Solutions}


\rhead{1/10/14}


\cfoot{\thepage\ of \pageref{LastPage}}


\title{Laminar Film \{Munson, Bird\}}

\maketitle

\subsection{Illustration}


\subsection{Assumptions}
\begin{enumerate}
\item Adiabatic Isothermal (no Energy Equation)
\item Steady State ($\frac{\partial}{\partial t}=0$)
\item Two Dimensional ($\frac{\partial}{\partial y}=0$)
\item Fully Developed ($\frac{\partial v_{z}}{\partial z}=0$)
\item Laminar ($\tau=-\mu\frac{\partial v_{z}}{\partial x}$)
\item Incompressible ($\frac{D\rho}{Dt}=0$)
\item No Slip ($\left.\vec{v}\right\rfloor _{\delta}=0$)
\item Uniform Surface Pressure ($p=p\left(z\right)$)
\end{enumerate}

\subsection{Continuity Equation}

\[
\frac{\partial\rho}{\partial t}+\nabla\cdot\left(\rho\vec{v}\right)=0\;\;\therefore\;\;\cancelto{0}{\frac{\partial\rho}{\partial t}+\vec{v}\cdot\nabla p}+\rho\nabla\cdot\vec{v}=0
\]


\[
\nabla\cdot\vec{v}=0
\]
\[
\frac{\partial v_{x}}{\partial x}+\cancelto{0}{\frac{\partial v_{z}}{\partial z}}=0\;\;\therefore\;\; v_{x}=c_{1}\;\;\&\;\;\left.v_{x}\right\rfloor _{\delta}=0\;\;\therefore\;\; v_{x}=0
\]



\subsection{Momentum Equation}

\[
\frac{\partial\rho\vec{v}}{\partial t}+\nabla\cdot\left(\rho\vec{v}\vec{v}\right)=-\nabla p-\nabla\cdot\boldsymbol{\tau}+\rho\vec{g}
\]


and applying to the x direction

\begin{multline*}
\rho\left(\cancelto{0}{\frac{\partial v_{x}}{\partial t}}+\cancelto{0}{v_{x}}\frac{\partial v_{x}}{\partial x}+v_{y}\cancelto{0}{\frac{\partial v_{x}}{\partial x}}+v_{x}\cancelto{0}{\frac{\partial v_{x}}{\partial x}}\right)\\
=-\frac{\partial p}{\partial x}+\rho g\sin\left(\theta\right)+\mu\left(\cancelto{0}{\frac{\partial^{2}v_{x}}{\partial x^{2}}}+\cancelto{0}{\frac{\partial^{2}v_{x}}{\partial y^{2}}}+\cancelto{0}{\frac{\partial^{2}v_{x}}{\partial z^{2}}}\right)
\end{multline*}


\[
\frac{\partial p}{\partial x}=\rho g\sin\left(\theta\right)
\]
'
\[
p=\rho g\sin\left(\theta\right)x+c_{2}\;\;\&\;\;\left.p\right\rfloor _{0}=p_{\infty}\;\;\therefore\;\; c_{2}=p_{\infty}\;\;\&\;\; p=p\left(x\right)
\]


now applying to the z direction.

\begin{multline*}
\rho\left(\cancelto{0}{\frac{\partial v_{z}}{\partial t}}+\cancelto{0}{v_{x}}\frac{\partial v_{z}}{\partial x}+v_{y}\cancelto{0}{\frac{\partial v_{z}}{\partial x}}+v_{x}\cancelto{0}{\frac{\partial v_{z}}{\partial x}}\right)\\
=-\cancelto{0}{\frac{\partial p}{\partial z}}+\rho g\cos\left(\theta\right)+\mu\left(\frac{\partial^{2}v_{z}}{\partial x^{2}}+\cancelto{0}{\frac{\partial^{2}v_{z}}{\partial y^{2}}}+\cancelto{0}{\frac{\partial^{2}v_{z}}{\partial z^{2}}}\right)
\end{multline*}


\[
\frac{\partial^{2}v_{z}}{\partial x^{2}}=-\frac{\rho g\cos\left(\theta\right)}{\mu}
\]


\[
\frac{\partial v_{z}}{\partial x}=-\frac{\rho g\cos\left(\theta\right)x}{\mu}+c_{3}\;\;\&\;\;\left.\frac{\partial v_{z}}{\partial x}\right\rfloor _{0}=0\;\;\therefore\;\; c_{3}=0
\]


\[
v_{z}=-\frac{\rho g\cos\left(\theta\right)}{2\mu}x^{2}+c_{4}\;\;\&\;\;\left.v_{z}\right\rfloor _{\delta}=0\;\;\therefore\;\; c_{4}=\frac{\rho g\cos\left(\theta\right)\delta^{2}}{2\mu}
\]


\[
v_{z}=\frac{\rho g\cos\left(\theta\right)\delta^{2}}{2\mu}\left[1-\left(\frac{x}{\delta}\right)^{2}\right]
\]


\[
\left\langle v_{z}\right\rangle =\frac{1}{\delta}\int_{0}^{\delta}\left\langle v_{z}\right\rangle dx
\]


\[
\left\langle v_{z}\right\rangle =\frac{\rho g\cos\left(\theta\right)\delta}{2\mu}\left[x-\frac{x^{3}}{3\delta^{2}}\right]_{0}^{\delta}=\frac{\rho g\cos\left(\theta\right)\delta}{2\mu}\left[\frac{2}{3}\delta\right]=\frac{\rho g\cos\left(\theta\right)\delta^{2}}{3\mu}
\]


\bibliographystyle{plain}
\bibliography{th}

\end{document}
